Working (and removed old/)

Multistep.v
@@ -1,17 +1,47 @@
 From Coq Require Import Arith.Arith.
-From Coq Require Import Lia.
 
-From Elo Require Import Util.
 From Elo Require Import Array.
-From Elo Require Import Map.
 From Elo Require Import Core.
 From Elo Require Import CoreExt.
-From Elo Require Import ValidAddresses.
-From Elo Require Import References.
-From Elo Require Import Soundness.
-From Elo Require Import Access.
-From Elo Require Import SafeSpawns.
-From Elo Require Import SMS.
+
+From Elo Require Import Definitions.
+
+From Elo Require Import PropertiesVAD.
+From Elo Require Import PropertiesACC.
+From Elo Require Import PropertiesSS.
+From Elo Require Import PropertiesSMS.
+
+(* ------------------------------------------------------------------------- *)
+(* multistep monotonic-nondecreasing                                         *)
+(* ------------------------------------------------------------------------- *)
+
+Lemma monotonic_nondecreasing_memory_length: forall m m' ths ths' tc,
+  m / ths ~~[tc]~~>* m' / ths' ->
+  #m <= #m'.
+Proof.
+  assert (forall m m' e t t',
+    m / t ==[e]==> m' / t' ->
+    #m <= #m'). {
+    intros. inv_mstep; eauto.
+    - rewrite add_increments_length. eauto.
+    - rewrite set_preserves_length. eauto.
+  }
+  intros. induction_multistep; trivial. inv_cstep; eauto.
+  eauto using Nat.le_trans.
+Qed.
+
+Lemma monotonic_nondecreasing_threads_length: forall m m' ths ths' tc,
+  m / ths ~~[tc]~~>* m' / ths' ->
+  #ths <= #ths'.
+Proof.
+  intros. induction_multistep; trivial. inv_cstep;
+  try rewrite add_increments_length; rewrite set_preserves_length;
+  eauto using Nat.le_trans.
+Qed.
+
+(* ------------------------------------------------------------------------- *)
+(* multistep preservation                                                    *)
+(* ------------------------------------------------------------------------- *)
 
 Theorem memory_value_multistep_preservation : forall m m' ths ths' tc,
   forall_memory m value ->
@@ -20,14 +50,14 @@ Theorem memory_value_multistep_preservation : forall m m' ths ths' tc,
 Proof.
   assert (forall t t' ad v T, t --[EF_Alloc ad v T]--> t' -> value v);
   assert (forall t t' ad v T, t --[EF_Write ad v T]--> t' -> value v);
-  try solve [intros; induction_step; eauto].
+  try solve [intros; induction_tstep; eauto].
   intros. induction_multistep; trivial.
-  inversion_cstep; eauto. inversion_mstep; eauto;
+  inv_cstep; eauto. inv_mstep; eauto;
   (eapply forall_array_add || eapply forall_array_set);
   eauto using value; autounfold with fall in *; eauto.
 Qed.
 
-Local Ltac destruct_multistep_IH :=
+Local Ltac destruct_for_multistep :=
   match goal with
   | IH : context C [_ -> forall_program _ _ _] |- _ =>
     destruct IH
@@ -39,7 +69,7 @@ Corollary valid_addresses_multistep_preservation : forall m m' ths ths' tc,
   forall_program m' ths' (valid_addresses m').
 Proof.
   intros. induction_multistep; trivial.
-  destruct_multistep_IH; eauto using valid_addresses_preservation.
+  destruct_for_multistep; eauto using valid_addresses_preservation.
 Qed.
 
 Theorem typing_multistep_preservation : forall m m' ths ths' tc,
@@ -49,8 +79,8 @@ Theorem typing_multistep_preservation : forall m m' ths ths' tc,
   forall_program m ths (consistently_typed_references m) ->
   m / ths ~~[tc]~~>* m' / ths' ->
   forall_program m' ths' well_typed_term /\
-    forall_program m' ths' (consistently_typed_references m') /\
-    m' extends m.
+    forall_program m' ths' (consistently_typed_references m')
+    (* /\ m' extends m *).
 Proof.
   (* TODO *)
 Admitted.
@@ -60,63 +90,33 @@ Corollary safe_spawns_multistep_preservation : forall m m' ths ths' tc,
   forall_program m ths well_typed_term ->
   forall_program m ths (consistently_typed_references m) ->
   (* --- *)
-  forall_program m ths SafeSpawns ->
+  forall_program m ths safe_spawns ->
   m / ths ~~[tc]~~>* m' / ths' ->
-  forall_program m' ths' SafeSpawns.
+  forall_program m' ths' safe_spawns.
 Proof.
   intros. induction_multistep; trivial.
   assert (forall_program m' ths' well_typed_term)
     by (eapply typing_multistep_preservation; eauto).
-  destruct_multistep_IH; eauto using safe_spawns_preservation.
+  destruct_for_multistep; eauto using safe_spawns_preservation.
 Qed.
 
-Theorem safe_memory_sharing_multistep_preservation : forall m m' ths ths' tc,
+Corollary safe_memory_sharing_multistep_preservation : forall m m' ths ths' tc,
   forall_memory m value ->
   forall_program m ths well_typed_term ->
   forall_program m ths (valid_addresses m) ->
   forall_program m ths (consistently_typed_references m) ->
-  forall_program m ths SafeSpawns ->
+  forall_program m ths safe_spawns ->
   (* --- *)
   safe_memory_sharing m ths ->
   m / ths ~~[tc]~~>* m' / ths' ->
   safe_memory_sharing m' ths'.
 Proof.
   intros. induction_multistep; trivial.
-  (* TODO *)
-  eapply (safe_memory_sharing_preservation m' m'' ths' ths''); eauto;
+  eapply (safe_memory_sharing_preservation m' m'' ths' ths'');
   eauto using memory_value_multistep_preservation,
               valid_addresses_multistep_preservation,
               safe_spawns_multistep_preservation;
   eapply typing_multistep_preservation; eauto.
-Qed.
-
-(* ------------------------------------------------------------------------- *)
-(*                                                                           *)
-(* ------------------------------------------------------------------------- *)
-
-
-Lemma monotonic_nondecreasing_memory_length: forall m m' ths ths' tc,
-  m / ths ~~[tc]~~>* m' / ths' ->
-  #m <= #m'.
-Proof.
-  assert (forall m m' e t t',
-    m / t ==[e]==> m' / t' ->
-    #m <= #m'). {
-    intros. inversion_mstep; try lia.
-    - rewrite add_increments_length. lia.
-    - eauto using Nat.eq_le_incl, set_preserves_length.
-  }
-  intros. induction_multistep; trivial. inversion_cstep; eauto.
-  eauto using Nat.le_trans.
-Qed.
-
-Lemma monotonic_nondecreasing_threads_length: forall m m' ths ths' tc,
-  m / ths ~~[tc]~~>* m' / ths' ->
-  #ths <= #ths'.
-Proof.
-  intros. induction_multistep; trivial. inversion_cstep;
-  try rewrite add_increments_length; rewrite set_preserves_length;
-  eauto using Nat.le_trans.
 Qed.
 
 Theorem not_access_multistep_preservation : forall m m' ths ths' tid ad tc,
@@ -124,7 +124,7 @@ Theorem not_access_multistep_preservation : forall m m' ths ths' tid ad tc,
   forall_program m ths (valid_addresses m) ->
   forall_program m ths well_typed_term ->
   forall_program m ths (consistently_typed_references m) ->
-  forall_program m ths SafeSpawns ->
+  forall_program m ths safe_spawns ->
   safe_memory_sharing m ths ->
   (* --- *)
   ad < #m ->
@@ -140,6 +140,32 @@ Proof.
               monotonic_nondecreasing_memory_length,
               monotonic_nondecreasing_threads_length,
               Nat.le_trans.
-  eapply typing_multistep_preservation; eauto.
+  (* TODO *)
+  - eapply valid_addresses_multistep_preservation; eauto.
+  - eapply valid_addresses_multistep_preservation; eauto.
+  - eapply typing_multistep_preservation; eauto.
+Qed.
+
+Definition valid_program m ths :=
+  (  forall_memory  m value
+  /\ forall_program m ths well_typed_term
+  /\ forall_program m ths (valid_addresses m)
+  /\ forall_program m ths (consistently_typed_references m)
+  /\ forall_program m ths safe_spawns
+  /\ safe_memory_sharing m ths).
+
+Corollary properties_preservation : forall m m' ths ths' tc,
+  valid_program m ths ->
+  m / ths ~~[tc]~~>* m' / ths' ->
+  valid_program m' ths'.
+Proof.
+  unfold valid_program.
+  intros * Hvp **. decompose record Hvp. split.
+  eapply memory_value_multistep_preservation; eauto. split.
+  eapply typing_multistep_preservation; eauto. split.
+  eapply valid_addresses_multistep_preservation; eauto. split.
+  eapply typing_multistep_preservation; eauto. split.
+  eapply safe_spawns_multistep_preservation; eauto.
+  eapply safe_memory_sharing_multistep_preservation; eauto.
 Qed.
 
