PropertiesACC.v
@@ -25,196 +25,305 @@ Qed.
 (* access inheritance                                                        *)
 (* ------------------------------------------------------------------------- *)
 
-Module Inheritance.
-  Lemma alt_acc_mem_set_inheritance : forall m t ad ad' vT,
-    ~ access ad' m t ->
-    (* --- *)
-    access ad m[ad' <- vT] t ->
-    access ad m t.
-  Proof.
-    intros * ? Hacc. induction Hacc; inv_nacc; eauto using access.
-    simpl_array. eauto using access.
-  Qed.
-End Inheritance.
+(* mem & subst ------------------------------------------------------------- *)
+
+Lemma acc_subst_inheritance : forall m x Tx t t' ad,
+  access ad m ([x := t'] t) ->
+  access ad m <{call <{fn x Tx t}> t'}>.
+Proof.
+  intros. induction t; eauto using access; simpl in *;
+  try (destruct string_eq_dec; eauto using access);
+  invc_acc; auto_specialize; do 2 inv_acc; eauto using access.
+Qed.
+
+Lemma acc_mem_add_inheritance : forall m t ad vT,
+  forall_memory m (valid_addresses m) ->
+  valid_addresses m t ->
+  (* --- *)
+  access ad (m +++ vT) t ->
+  access ad m t.
+Proof.
+  intros * Hmvad Hvad Hacc.
+  assert (Hnacc : ~ access (#m) m t) by eauto using nacc_vad_length.
+  clear Hvad. induction Hacc; inv_nacc; eauto using access.
+  decompose sum (lt_eq_lt_dec ad' (#m)); subst; eauto;
+  simpl_array; eauto using access. simpl in *. inv_acc.
+Qed.
+
+Lemma acc_mem_set_inheritance : forall m t ad ad' v T,
+  ~ access ad m v ->
+  (* --- *)
+  access ad m[ad' <- (v, T)] t ->
+  access ad m t.
+Proof.
+  intros * Hnacc Hacc. remember (m[ad' <- (v, T)]) as m'.
+  induction Hacc; inv Heqm'; eauto using access.
+  match goal with |- access _ _ <{& ?ad :: _}> => rename ad into ad'' end.
+  destruct (nat_eq_dec ad' ad''); subst; try (simpl_array; eauto using access);
+  destruct (nat_eq_dec ad'' ad); subst; eauto using access;
+  rewrite (get_set_eq memory_default) in IHHacc. 1: contradiction.
+  decompose sum (lt_eq_lt_dec ad'' (#m)); subst; trivial;
+  simpl_array; simpl in *; inv_acc.
+Qed.
+
+Lemma alt_acc_mem_set_inheritance : forall m t ad ad' vT,
+  ~ access ad' m t ->
+  (* --- *)
+  access ad m[ad' <- vT] t ->
+  access ad m t.
+Proof.
+  intros * ? Hacc. induction Hacc; inv_nacc; eauto using access.
+  simpl_array. eauto using access.
+Qed.
+
+(* tstep ------------------------------------------------------------------- *)
+
+Lemma acc_tstep_none_inheritance  : forall m t t' ad,
+  access ad m t' ->
+  t --[EF_None]--> t' ->
+  access ad m t.
+Proof.
+  intros. induction_tstep; eauto using access, acc_subst_inheritance;
+  inv_acc; eauto using access.
+Qed.
+
+Lemma acc_tstep_alloc_inheritance : forall m t t' ad v T,
+  forall_memory m (valid_addresses m) ->
+  valid_addresses m t ->
+  (* --- *)
+  ad < #m ->
+  access ad (m +++ (v, T)) t' ->
+  t --[EF_Alloc (#m) v T]--> t' ->
+  access ad m t.
+Proof.
+  intros. induction_tstep; inv_vad; inv_acc;
+  eauto using access, acc_mem_add_inheritance.
+  simpl_array. eauto using access, acc_mem_add_inheritance.
+Qed.
+
+Lemma acc_tstep_read_inheritance : forall m t t' ad ad',
+  access ad m t' ->
+  t --[EF_Read ad' m[ad'].tm]--> t' ->
+  access ad m t.
+Proof.
+  intros. induction_tstep; try inv_acc; eauto using access.
+  destruct (nat_eq_dec ad' ad); subst; eauto using access.
+Qed.
+
+Lemma acc_tstep_write_inheritance : forall m t t' ad ad' v T,
+  access ad m[ad' <- (v, T)] t' ->
+  t --[EF_Write ad' v T]--> t' ->
+  access ad m t.
+Proof.
+  intros. induction_tstep; inv_acc; eauto using access;
+  destruct (acc_dec ad m v); eauto using access, acc_mem_set_inheritance;
+  assert (forall t t', t --[EF_Write ad' v T]--> t' -> access ad m t)
+    by (intros; induction_tstep; eauto using access);
+  eauto using access.
+Qed.
+
+Lemma acc_tstep_spawn_inheritance : forall m t t' block ad,
+  access ad m t' ->
+  t --[EF_Spawn block]--> t' ->
+  access ad m t.
+Proof.
+  intros. induction_tstep; inv_acc; eauto using access.
+Qed.
+
+(* mstep ------------------------------------------------------------------- *)
+
+Corollary acc_mstep_inheritance : forall m m' t t' ad e,
+  forall_memory m (valid_addresses m) ->
+  valid_addresses m t ->
+  (* --- *)
+  ad < #m ->
+  access ad m' t' ->
+  m / t ==[e]==> m' / t' ->
+  access ad m t.
+Proof.
+  intros. inv_mstep;
+  eauto using acc_tstep_none_inheritance,
+              acc_tstep_alloc_inheritance,
+              acc_tstep_read_inheritance,
+              acc_tstep_write_inheritance.
+Qed.
 
 (* ------------------------------------------------------------------------- *)
 (* not-access preservation                                                   *)
 (* ------------------------------------------------------------------------- *)
 
-Module PreservationNACC.
-  (* subst & mem ----------------------------------------------------------- *)
+(* subst & mem ------------------------------------------------------------- *)
 
-  Lemma nacc_subst_preservation : forall m t tx ad x,
-    ~ access ad m t ->
-    ~ access ad m tx ->
-    ~ access ad m ([x := tx] t).
-  Proof.
-    intros. induction t; simpl; eauto using access;
-    try inv_nacc; eauto with acc;
-    destruct string_eq_dec; subst; eauto with acc.
-  Qed.
+Lemma nacc_subst_preservation : forall m t tx ad x,
+  ~ access ad m t ->
+  ~ access ad m tx ->
+  ~ access ad m ([x := tx] t).
+Proof.
+  intros. induction t; simpl; eauto using access;
+  try inv_nacc; eauto with acc;
+  destruct string_eq_dec; subst; eauto with acc.
+Qed.
 
-  Lemma nacc_mem_add_preservation : forall m t ad vT,
-    ~ access (#m) m t ->
-    (* --- *)
-    ~ access ad m t ->
-    ~ access ad (m +++ vT) t.
-  Proof.
-    intros ** Hacc. induction Hacc; inv_nacc; inv_nacc; eauto.
-    decompose sum (lt_eq_lt_dec ad' (#m)); subst; simpl_array; eauto.
-  Qed.
+Lemma nacc_mem_add_preservation : forall m t ad vT,
+  ~ access (#m) m t ->
+  (* --- *)
+  ~ access ad m t ->
+  ~ access ad (m +++ vT) t.
+Proof.
+  intros ** Hacc. induction Hacc; inv_nacc; inv_nacc; eauto.
+  decompose sum (lt_eq_lt_dec ad' (#m)); subst; simpl_array; eauto.
+Qed.
 
-  Lemma nacc_mem_set_preservation : forall m t ad ad' v T,
-    ~ access ad m v ->
-    ~ access ad m t ->
-    ~ access ad m[ad' <- (v, T)] t.
-  Proof.
-    assert (forall m ad ad' v,
-      access ad m[ad' <- v] m[ad' <- v][ad'].tm -> ad' < #m). {
-        intros * H. decompose sum (lt_eq_lt_dec ad' (#m)); subst; trivial;
-        simpl_array; simpl in *; inv_acc.
-    }
-    (* main proof *)
-    intros ** Hacc. induction Hacc; eauto using access.
-    match goal with _ : _ <> ?ad |- _ => rename ad into ad'' end. 
-    destruct (nat_eq_dec ad' ad''); subst;
-    try (assert (ad'' < #m) by eauto);
-    simpl_array; eauto using access.
-  Qed.
+Lemma nacc_mem_set_preservation : forall m t ad ad' v T,
+  ~ access ad m v ->
+  ~ access ad m t ->
+  ~ access ad m[ad' <- (v, T)] t.
+Proof.
+  assert (forall m ad ad' v,
+    access ad m[ad' <- v] m[ad' <- v][ad'].tm -> ad' < #m). {
+      intros * H. decompose sum (lt_eq_lt_dec ad' (#m)); subst; trivial;
+      simpl_array; simpl in *; inv_acc.
+  }
+  (* main proof *)
+  intros ** Hacc. induction Hacc; eauto using access.
+  match goal with _ : _ <> ?ad |- _ => rename ad into ad'' end. 
+  destruct (nat_eq_dec ad' ad''); subst;
+  try (assert (ad'' < #m) by eauto);
+  simpl_array; eauto using access.
+Qed.
 
-  Lemma alt_nacc_mem_set_preservation : forall m t ad ad' vT,
-    ~ access ad' m t ->
-    (* --- *)
-    ~ access ad m t ->
-    ~ access ad m[ad' <- vT] t.
-  Proof.
-    intros ** Hacc.
-    induction Hacc; inv_nacc; inv_nacc; eauto using access.
-    simpl_array. eauto.
-  Qed.
+Lemma alt_nacc_mem_set_preservation : forall m t ad ad' vT,
+  ~ access ad' m t ->
+  (* --- *)
+  ~ access ad m t ->
+  ~ access ad m[ad' <- vT] t.
+Proof.
+  intros ** Hacc.
+  induction Hacc; inv_nacc; inv_nacc; eauto using access.
+  simpl_array. eauto.
+Qed.
 
-  (* tstep ----------------------------------------------------------------- *)
+(* tstep ------------------------------------------------------------------- *)
 
-  Lemma nacc_tstep_none_preservation : forall m t t' ad,
-    ~ access ad m t ->
-    t --[EF_None]--> t' ->
-    ~ access ad m t'.
-  Proof.
-    intros. induction_tstep; inv_nacc; eauto with acc.
-    inv_nacc. eauto using nacc_subst_preservation.
-  Qed.
+Lemma nacc_tstep_none_preservation : forall m t t' ad,
+  ~ access ad m t ->
+  t --[EF_None]--> t' ->
+  ~ access ad m t'.
+Proof.
+  intros. induction_tstep; inv_nacc; eauto with acc.
+  inv_nacc. eauto using nacc_subst_preservation.
+Qed.
 
-  Lemma nacc_tstep_alloc_preservation : forall m t t' ad v T,
-    forall_memory m (valid_addresses m) ->
-    valid_addresses m t ->
-    (* --- *)
-    ad < #m ->
-    ~ access ad m t ->
-    t --[EF_Alloc (#m) v T]--> t' ->
-    ~ access ad (m +++ (v, T)) t'.
-  Proof.
-    intros. induction_tstep; inv_vad; inv_nacc;
-    eauto using nacc_mem_add_preservation, nacc_vad_length with acc.
-    eapply nacc_ad.
-    - intros ?. subst. eauto.
-    - simpl_array. eauto using nacc_mem_add_preservation, nacc_vad_length.
-  Qed.
+Lemma nacc_tstep_alloc_preservation : forall m t t' ad v T,
+  forall_memory m (valid_addresses m) ->
+  valid_addresses m t ->
+  (* --- *)
+  ad < #m ->
+  ~ access ad m t ->
+  t --[EF_Alloc (#m) v T]--> t' ->
+  ~ access ad (m +++ (v, T)) t'.
+Proof.
+  intros. induction_tstep; inv_vad; inv_nacc;
+  eauto using nacc_mem_add_preservation, nacc_vad_length with acc.
+  eapply nacc_ad.
+  - intros ?. subst. eauto.
+  - simpl_array. eauto using nacc_mem_add_preservation, nacc_vad_length.
+Qed.
 
-  Lemma nacc_tstep_read_preservation : forall m t t' ad ad',
-    ~ access ad m t ->
-    t --[EF_Read ad' m[ad'].tm]--> t' ->
-    ~ access ad m t'.
-  Proof.
-    intros. induction_tstep; inv_nacc; eauto with acc.
-    inv_nacc. assumption.
-  Qed.
+Lemma nacc_tstep_read_preservation : forall m t t' ad ad',
+  ~ access ad m t ->
+  t --[EF_Read ad' m[ad'].tm]--> t' ->
+  ~ access ad m t'.
+Proof.
+  intros. induction_tstep; inv_nacc; eauto with acc.
+  inv_nacc. assumption.
+Qed.
 
-  Lemma nacc_tstep_write_preservation : forall m t t' ad ad' v T,
-    ~ access ad m t ->
-    t --[EF_Write ad' v T]--> t' ->
-    ~ access ad m[ad' <- (v, T)] t'.
-  Proof.
-    intros.
-    assert (~ access ad m v) by eauto using nacc_tstep_write_value.
-    induction_tstep; inv_nacc; eauto using nacc_mem_set_preservation with acc.
-  Qed.
+Lemma nacc_tstep_write_preservation : forall m t t' ad ad' v T,
+  ~ access ad m t ->
+  t --[EF_Write ad' v T]--> t' ->
+  ~ access ad m[ad' <- (v, T)] t'.
+Proof.
+  intros.
+  assert (~ access ad m v) by eauto using nacc_tstep_write_value.
+  induction_tstep; inv_nacc; eauto using nacc_mem_set_preservation with acc.
+Qed.
 
-  Lemma nacc_tstep_spawn_preservation : forall m t t' block ad,
-    ~ access ad m t ->
-    t --[EF_Spawn block]--> t' ->
-    ~ access ad m t'.
-  Proof.
-    intros. induction_tstep; eauto with acc; inv_nacc; eauto with acc.
-  Qed.
+Lemma nacc_tstep_spawn_preservation : forall m t t' block ad,
+  ~ access ad m t ->
+  t --[EF_Spawn block]--> t' ->
+  ~ access ad m t'.
+Proof.
+  intros. induction_tstep; eauto with acc; inv_nacc; eauto with acc.
+Qed.
 
-  (* mstep ----------------------------------------------------------------- *)
+(* mstep ------------------------------------------------------------------- *)
 
-  Corollary nacc_mstep_preservation : forall m m' t t' ad e,
-    forall_memory m (valid_addresses m) ->
-    valid_addresses m t ->
-    (* --- *)
-    ad < #m ->
-    ~ access ad m t ->
-    m / t ==[e]==> m' / t' ->
-    ~ access ad m' t'.
-  Proof.
-    intros. inv_mstep;
-    eauto using nacc_tstep_none_preservation,
-                nacc_tstep_alloc_preservation,
-                nacc_tstep_read_preservation,
-                nacc_tstep_write_preservation.
-  Qed.
+Corollary nacc_mstep_preservation : forall m m' t t' ad e,
+  forall_memory m (valid_addresses m) ->
+  valid_addresses m t ->
+  (* --- *)
+  ad < #m ->
+  ~ access ad m t ->
+  m / t ==[e]==> m' / t' ->
+  ~ access ad m' t'.
+Proof.
+  intros. inv_mstep;
+  eauto using nacc_tstep_none_preservation,
+              nacc_tstep_alloc_preservation,
+              nacc_tstep_read_preservation,
+              nacc_tstep_write_preservation.
+Qed.
 
-  (* cstep ----------------------------------------------------------------- *)
+(* cstep ------------------------------------------------------------------- *)
 
-  Local Lemma uacc_tstep_write_requirement : forall m t t' ad v T,
-    well_typed_term t ->
-    t --[EF_Write ad v T]--> t' ->
-    unsafe_access ad m t.
-  Proof.
-    intros * [T' ?] **. generalize dependent T'.
-    induction_tstep; intros; inv_type; eauto using unsafe_access.
-    inv_type. eauto using unsafe_access.
-  Qed.
+Local Lemma uacc_tstep_write_requirement : forall m t t' ad v T,
+  well_typed_term t ->
+  t --[EF_Write ad v T]--> t' ->
+  unsafe_access ad m t.
+Proof.
+  intros * [T' ?] **. generalize dependent T'.
+  induction_tstep; intros; inv_type; eauto using unsafe_access.
+  inv_type. eauto using unsafe_access.
+Qed.
 
-  Lemma nacc_untouched_threads_preservation : forall m m' ths tid tid' t' ad e,
-    forall_memory m (valid_addresses m) ->
-    forall_threads ths (valid_addresses m) ->
-    forall_threads ths well_typed_term ->
-    safe_memory_sharing m ths ->
-    (* --- *)
-    tid <> tid' ->
-    tid' < #ths ->
-    ~ access ad m ths[tid'] ->
-    m / ths[tid] ==[e]==> m' / t' ->
-    ~ access ad m' ths[tid'].
-  Proof.
-    intros * ? ? ? Hsms **. rename ad into ad'. invc_mstep;
-    eauto using nacc_mem_add_preservation, nacc_vad_length.
-    eapply alt_nacc_mem_set_preservation; eauto.
-    assert (unsafe_access ad m ths[tid])
-      by eauto using uacc_tstep_write_requirement.
-    intros ?. eapply (Hsms tid tid'); eauto.
-  Qed.
+Lemma nacc_untouched_threads_preservation : forall m m' ths tid tid' t' ad e,
+  forall_memory m (valid_addresses m) ->
+  forall_threads ths (valid_addresses m) ->
+  forall_threads ths well_typed_term ->
+  safe_memory_sharing m ths ->
+  (* --- *)
+  tid <> tid' ->
+  tid' < #ths ->
+  ~ access ad m ths[tid'] ->
+  m / ths[tid] ==[e]==> m' / t' ->
+  ~ access ad m' ths[tid'].
+Proof.
+  intros * ? ? ? Hsms **. rename ad into ad'. invc_mstep;
+  eauto using nacc_mem_add_preservation, nacc_vad_length.
+  eapply alt_nacc_mem_set_preservation; eauto.
+  assert (unsafe_access ad m ths[tid])
+    by eauto using uacc_tstep_write_requirement.
+  intros ?. eapply (Hsms tid tid'); eauto.
+Qed.
 
-  Corollary nacc_cstep_preservation : forall m m' ths ths' tid tid' ad e,
-    forall_memory m (valid_addresses m) ->
-    forall_threads ths (valid_addresses m) ->
-    forall_threads ths well_typed_term ->
-    safe_memory_sharing m ths ->
-    (* --- *)
-    ad < #m ->
-    tid < #ths ->
-    ~ access ad m ths[tid] ->
-    m / ths ~~[tid', e]~~> m' / ths' ->
-    ~ access ad m' ths'[tid].
-  Proof.
-    intros. invc_cstep; destruct (nat_eq_dec tid tid'); subst; simpl_array;
-    eauto using nacc_tstep_spawn_preservation,
-                nacc_mstep_preservation,
-                nacc_untouched_threads_preservation.
-  Qed.
-End PreservationNACC.
+Corollary nacc_cstep_preservation : forall m m' ths ths' tid tid' ad e,
+  forall_memory m (valid_addresses m) ->
+  forall_threads ths (valid_addresses m) ->
+  forall_threads ths well_typed_term ->
+  safe_memory_sharing m ths ->
+  (* --- *)
+  ad < #m ->
+  tid < #ths ->
+  ~ access ad m ths[tid] ->
+  m / ths ~~[tid', e]~~> m' / ths' ->
+  ~ access ad m' ths'[tid].
+Proof.
+  intros. invc_cstep; destruct (nat_eq_dec tid tid'); subst; simpl_array;
+  eauto using nacc_tstep_spawn_preservation,
+              nacc_mstep_preservation,
+              nacc_untouched_threads_preservation.
+Qed.
 
 (* ------------------------------------------------------------------------- *)
 (* misc. properties                                                          *)
@@ -231,6 +340,6 @@ Proof.
   destruct (nat_eq_dec ad' ad''); subst; eauto using access.
   simpl_array. eapply acc_mem; trivial.
   destruct (acc_dec ad' m m[ad''].tm); trivial. exfalso.
-  eapply (PreservationNACC.alt_nacc_mem_set_preservation _ _ ad ad'); eauto.
+  eapply (alt_nacc_mem_set_preservation _ _ ad ad'); eauto.
 Qed.
 
