PropertiesSMS.v
@@ -1,37 +1,41 @@
+From Elo Require Import Util.
+From Elo Require Import Core.
+From Elo Require Import Array.
+From Elo Require Import Map.
+From Elo Require Import CoreExt.
+
+From Elo Require Import Definitions.
+
+From Elo Require Import PropertiesVAD.
+From Elo Require Import PropertiesCTR.
+From Elo Require Import PropertiesACC.
+From Elo Require Import PropertiesUACC.
+From Elo Require Import PropertiesSS.
 
 (* ------------------------------------------------------------------------- *)
-(* acc, uacc & memtyp                                                        *)
+(* misc. properties                                                          *)
 (* ------------------------------------------------------------------------- *)
 
-(* If the access is unsafe, then the memtyp is mutable. *)
-Local Lemma uacc_then_memtyp_mut : forall m t ad,
-  forall_memory m (consistently_typed_references m) ->
-  consistently_typed_references m t ->
-  (* --- *)
-  unsafe_access ad m t ->
-  exists T, m[ad].typ = <{{&T}}>.
-Proof.
-  intros * ? ? Huacc. induction Huacc; inversion_ctr; eauto.
-Qed.
-
-(* If the memtyp is mutable, then the access is unsafe. *)
-Local Lemma memtyp_mut_then_uacc : forall m t ad T,
+(* If there is access: *)
+(* The access is unsafe if and only if the memtyp is mutable. *)
+Lemma uacc_iff_memtyp_mut : forall m t ad,
   forall_memory m value ->
   forall_memory m (consistently_typed_references m) ->
   consistently_typed_references m t ->
-  (* --- *)
-  m[ad].typ = <{{&T}}> ->
   access ad m t ->
-  unsafe_access ad m t.
+  (* --- *)
+  unsafe_access ad m t <-> (exists T, m[ad].typ = <{{&T}}>).
 Proof.
-  intros * ? ? ? Heq Hacc.
-  induction Hacc; inversion_ctr; eauto using unsafe_access.
-  - exfalso. eauto using immutable_reference_then_nuacc.
-  - rewrite Heq in *. discriminate.
+  intros * ? ? ? Hacc. split.
+  - intros Huacc. clear Hacc. induction Huacc; inv_ctr; eauto.
+  - intros [T Heq].
+    induction Hacc; inv_ctr; eauto using unsafe_access.
+    + exfalso. eauto using nuacc_from_immutable_type.
+    + rewrite Heq in *. discriminate.
 Qed.
 
 (* If one access is unsafe, then all accesses are unsafe. *)
-Local Corollary uacc_from_association : forall m t t' ad,
+Corollary uacc_from_association : forall m t t' ad,
   forall_memory m value ->
   forall_memory m (consistently_typed_references m) ->
   consistently_typed_references m t ->
@@ -42,8 +46,8 @@ Local Corollary uacc_from_association : forall m t t' ad,
   unsafe_access ad m t.
 Proof.
   intros.
-  assert (exists T, m[ad].typ = <{{&T}}>) as [? ?];
-  eauto using uacc_then_memtyp_mut, memtyp_mut_then_uacc.
+  eapply uacc_iff_memtyp_mut; eauto.
+  eapply uacc_iff_memtyp_mut; eauto using uacc_then_acc.
 Qed.
 
 (* ------------------------------------------------------------------------- *)
@@ -63,8 +67,8 @@ Proof.
     unsafe_access ad m t
   ). {
     intros. generalize dependent T.
-    induction_step; intros; inversion_type; eauto using unsafe_access.
-    inversion_type. eauto using unsafe_access.
+    induction_tstep; intros; inv_type; eauto using unsafe_access.
+    inv_type. eauto using unsafe_access.
   }
   (* main proof *)
   intros * Hneq Htype Hsms ? Hacc.
@@ -85,7 +89,7 @@ Local Ltac destruct_sms ths tid tid1 tid2 :=
   destruct (nat_eq_dec tid tid1), (nat_eq_dec tid tid2); subst;
   try contradiction.
 
-Local Lemma sms_tstep_none_preservation : forall m t ths tid,
+Lemma sms_tstep_none_preservation : forall m t ths tid,
   safe_memory_sharing m ths ->
   ths[tid] --[EF_None]--> t ->
   safe_memory_sharing m ths[tid <- t].
@@ -94,7 +98,7 @@ Proof.
   eauto using acc_tstep_none_inheritance, nuacc_tstep_none_preservation.
 Qed.
 
-Local Lemma sms_tstep_alloc_preservation : forall m t v ths tid T,
+Lemma sms_tstep_alloc_preservation : forall m t v ths tid T,
   forall_memory m (valid_addresses m) ->
   forall_threads ths (valid_addresses m) ->
   (* --- *)
@@ -104,19 +108,19 @@ Local Lemma sms_tstep_alloc_preservation : forall m t v ths tid T,
 Proof.
   intros ** tid1 tid2 ** Huacc.
   assert (Hvac : forall_threads ths (valid_accesses m))
-    by eauto using forall_threads_vad_then_vac.
+    by (intros ?; eauto using vad_then_vac).
   assert (forall tid, ~ unsafe_access (#m) m ths[tid])
-    by (intros * F; eapply uacc_then_acc in F; eapply Hvac in F; eauto).
-  autounfold with vac in Hvac. 
+    by eauto using nuacc_vad_length.
+  autounfold with vac in Hvac.
   eapply uacc_then_acc in Huacc as ?. contradict Huacc.
   destruct_sms ths tid tid1 tid2; simpl_array;
-  eauto 7 using nuacc_tstep_alloc_preservation,
+  eauto 6 using nuacc_tstep_alloc_preservation,
                 acc_tstep_alloc_inheritance,
                 nuacc_mem_add_preservation,
                 acc_mem_add_inheritance.
 Qed.
 
-Local Lemma sms_tstep_read_preservation : forall m t ad ths tid,
+Lemma sms_tstep_read_preservation : forall m t ad ths tid,
   forall_memory m value ->
   forall_threads ths well_typed_term ->
   forall_threads ths (consistently_typed_references m) ->
@@ -130,7 +134,7 @@ Proof.
   eauto using acc_tstep_read_inheritance, nuacc_tstep_read_preservation.
 Qed.
 
-Local Lemma sms_tstep_write_preservation : forall m ths t tid ad v T,
+Lemma sms_tstep_write_preservation : forall m ths t tid ad v T,
   forall_threads ths well_typed_term ->
   (* --- *)
   safe_memory_sharing m ths ->
@@ -149,31 +153,31 @@ Proof.
     alt_acc_mem_set_inheritance.
 Qed.
 
-Local Lemma sms_tstep_spawn_preservation : forall m ths t block tid,
+Lemma sms_tstep_spawn_preservation : forall m ths t block tid,
   forall_memory m value ->
   forall_memory m (valid_addresses m) ->
   forall_memory m (consistently_typed_references m) ->
   forall_threads ths (valid_addresses m) ->
   forall_threads ths (consistently_typed_references m) ->
-  forall_threads ths SafeSpawns ->
+  forall_threads ths safe_spawns ->
   (* --- *)
   safe_memory_sharing m ths ->
   ths[tid] --[EF_Spawn block]--> t ->
   safe_memory_sharing m (ths[tid <- t] +++ block).
 Proof.
   intros ** tid1 tid2 **.
-  assert (~ unsafe_access ad m block) by eauto using nuacc_spawn_block .
+  assert (~ unsafe_access ad m block) by eauto using nuacc_spawn_block.
   assert (consistently_typed_references m block) by eauto using ctr_spawn_block.
   destruct_sms ths tid tid1 tid2;
   decompose sum (lt_eq_lt_dec tid1 (#ths)); subst; simpl_array;
   decompose sum (lt_eq_lt_dec tid2 (#ths)); subst; simpl_array;
-  try solve [inversion_step | inv_acc | intros ?; inv_uacc];
+  try solve [inv_step | inv_acc | intros ?; inv_uacc];
   eauto using uacc_from_association,
     nuacc_tstep_spawn_preservation,
     acc_tstep_spawn_inheritance.
 Qed.
 
-Local Corollary sms_mstep_preservation : forall m m' t e ths tid,
+Corollary sms_mstep_preservation : forall m m' t e ths tid,
   forall_memory m value ->
   forall_memory m (valid_addresses m) ->
   forall_threads ths (valid_addresses m) ->
@@ -184,30 +188,27 @@ Local Corollary sms_mstep_preservation : forall m m' t e ths tid,
   m / ths[tid] ==[e]==> m' / t ->
   safe_memory_sharing m' ths[tid <- t].
 Proof.
-  intros. inversion_mstep;
+  intros. inv_mstep;
   eauto using sms_tstep_none_preservation,
-    sms_tstep_alloc_preservation,
-    sms_tstep_read_preservation,
-    sms_tstep_write_preservation.
+              sms_tstep_alloc_preservation,
+              sms_tstep_read_preservation,
+              sms_tstep_write_preservation.
 Qed.
 
-(* ------------------------------------------------------------------------- *)
+(* safe-memory-sharing preservation ---------------------------------------- *)
 
 Theorem safe_memory_sharing_preservation : forall m m' ths ths' tid e,
   forall_memory m value ->
   forall_program m ths (valid_addresses m) ->
   forall_program m ths well_typed_term ->
   forall_program m ths (consistently_typed_references m) ->
-  forall_program m ths SafeSpawns ->
+  forall_program m ths safe_spawns ->
   (* --- *)
   safe_memory_sharing m ths ->
   m / ths ~~[tid, e]~~> m' / ths' ->
   safe_memory_sharing m' ths'.
 Proof.
   intros * ? [? ?] [_ ?] [? ?] [_ ?] **.
-  assert (forall_threads ths (valid_accesses m))
-    by eauto using forall_threads_vad_then_vac.
-  inversion_clear_cstep;
-  eauto using sms_tstep_spawn_preservation, sms_mstep_preservation.
+  invc_cstep; eauto using sms_tstep_spawn_preservation, sms_mstep_preservation.
 Qed.
 
