PropertiesUACC.v
@@ -9,99 +9,104 @@ From Elo Require Import Definitions.
 From Elo Require Import PropertiesACC.
 
 (* ------------------------------------------------------------------------- *)
+(* misc. properties                                                          *)
+(* ------------------------------------------------------------------------- *)
+
+Corollary nuacc_vad_length : forall m t,
+  forall_memory m (valid_addresses m) ->
+  valid_addresses m t ->
+  ~ unsafe_access (#m) m t.
+Proof.
+  eauto using nacc_then_nuacc, nacc_vad_length.
+Qed.
+
+(* ------------------------------------------------------------------------- *)
 (* unsafe-access inheritance                                                 *)
 (* ------------------------------------------------------------------------- *)
 
-Module InheritanceUACC.
-  Lemma uacc_mem_add_inheritance : forall m t ad vT,
-    ~ access (#m) m t ->
-    (* --- *)
-    unsafe_access ad (m +++ vT) t ->
-    unsafe_access ad m t.
-  Proof.
-    intros * ? Huacc.
-    induction Huacc; inv_nacc; eauto using unsafe_access.
-    eapply uacc_mem; trivial.
-    decompose sum (lt_eq_lt_dec ad' (#m)); subst; simpl_array; eauto.
-  Qed.
+Lemma uacc_mem_add_inheritance : forall m t ad vT,
+  ~ access (#m) m t ->
+  (* --- *)
+  unsafe_access ad (m +++ vT) t ->
+  unsafe_access ad m t.
+Proof.
+  intros * ? Huacc.
+  induction Huacc; inv_nacc; eauto using unsafe_access.
+  eapply uacc_mem; trivial.
+  decompose sum (lt_eq_lt_dec ad' (#m)); subst; simpl_array; eauto.
+Qed.
 
-  Lemma uacc_mem_set_inheritance : forall m t ad ad' vT,
-    ~ access ad' m t ->
-    (* --- *)
-    unsafe_access ad m[ad' <- vT] t ->
-    unsafe_access ad m t.
-  Proof.
-    intros * ? Huacc.
-    induction Huacc; inv_nacc; eauto using unsafe_access.
-    simpl_array. eauto using unsafe_access.
-  Qed.
+Lemma uacc_mem_set_inheritance : forall m t ad ad' vT,
+  ~ access ad' m t ->
+  (* --- *)
+  unsafe_access ad m[ad' <- vT] t ->
+  unsafe_access ad m t.
+Proof.
+  intros * ? Huacc.
+  induction Huacc; inv_nacc; eauto using unsafe_access.
+  simpl_array. eauto using unsafe_access.
+Qed.
 
-  Lemma uacc_tstep_spawn_inheritance : forall m t t' block ad,
-    unsafe_access ad m t' ->
-    t --[EF_Spawn block]--> t' ->
-    unsafe_access ad m t.
-  Proof.
-    intros. induction_tstep; inv_uacc; eauto using unsafe_access.
-  Qed.
-End InheritanceUACC.
+Lemma uacc_tstep_spawn_inheritance : forall m t t' block ad,
+  unsafe_access ad m t' ->
+  t --[EF_Spawn block]--> t' ->
+  unsafe_access ad m t.
+Proof.
+  intros. induction_tstep; inv_uacc; eauto using unsafe_access.
+Qed.
 
 (* ------------------------------------------------------------------------- *)
 (* not-unsafe-access preservation                                            *)
 (* ------------------------------------------------------------------------- *)
 
-Local Lemma nuacc_subst_preservation : forall m t tx ad x,
+(* subst & mem ------------------------------------------------------------- *)
+
+Lemma nuacc_subst_preservation : forall m t tx ad x,
   ~ unsafe_access ad m t ->
   ~ unsafe_access ad m tx ->
   ~ unsafe_access ad m ([x := tx] t).
 Proof.
-  intros. intros ?. induction t; eauto; simpl in *;
-  try (destruct string_eq_dec; eauto);
-  inv_uacc; inv_nuacc; eauto.
+  intros ** ?. induction t; eauto; simpl in *;
+  try (destruct string_eq_dec); eauto; inv_uacc; inv_nuacc; eauto.
 Qed.
 
 Lemma nuacc_mem_add_preservation  : forall m t ad vT,
   ~ unsafe_access (#m) m t ->
+  (* --- *)
   ~ unsafe_access ad m t ->
   ~ unsafe_access ad (m +++ vT) t.
 Proof.
-  intros. intros Huacc. induction Huacc; inv_nuacc; eauto using unsafe_access.
-  decompose sum (lt_eq_lt_dec ad' (#m)); subst; simpl_array; simpl in *;
-  try inv_uacc; eauto using unsafe_access.
-  assert (#m <> ad') by (intros F; subst; eauto).
-  inv_nuacc. eauto.
+  intros ** Huacc. induction Huacc; inv_nuacc; eauto using unsafe_access.
+  decompose sum (lt_eq_lt_dec ad' (#m)); subst; simpl_array;
+  simpl in *; eauto using unsafe_access; inv_nuacc; eauto. inv_uacc.
 Qed.
 
 Lemma nuacc_mem_set_preservation : forall m t ad ad' v T,
   ~ unsafe_access ad m v ->
+  (* --- *)
   ~ unsafe_access ad m t ->
   ~ unsafe_access ad m[ad' <- (v, T)] t.
 Proof.
-  assert (forall m ad ad' v T,
-    unsafe_access ad m[ad' <- (v, T)] m[ad' <- (v, T)][ad'].tm -> ad' < #m). {
-      intros * H. decompose sum (lt_eq_lt_dec ad' (#m)); subst; trivial;
-      simpl_array; simpl in *; inv_uacc.
+  assert (H : forall m m' ad ad', unsafe_access ad m m'[ad'].tm -> ad' < #m'). {
+    intros * H. decompose sum (lt_eq_lt_dec ad' (#m')); subst; trivial;
+    simpl_array; simpl in *; inv_uacc.
   }
   (* main proof *)
-  intros * ? ? Huacc. induction Huacc; eauto using unsafe_access.
+  intros ** Huacc. induction Huacc; eauto using unsafe_access.
   match goal with _ : _ <> ?ad |- _ => rename ad into ad'' end. 
-  destruct (nat_eq_dec ad' ad''); subst;
-  try (assert (ad'' < #m) by eauto);
-  simpl_array; eauto using unsafe_access.
+  eapply H in Huacc. rewrite set_preserves_length in Huacc.
+  destruct (nat_eq_dec ad' ad''); subst; simpl_array; eauto using unsafe_access.
 Qed.
-
-(* alternative for mem_set ------------------------------------------------- *)
 
 Lemma alt_nuacc_mem_set_preservation : forall m t ad ad' vT,
   ~ unsafe_access ad' m t ->
+  (* --- *)
   ~ unsafe_access ad m t ->
   ~ unsafe_access ad m[ad' <- vT] t.
 Proof.
-  intros * ? ? Huacc.
-  induction Huacc; inv_nuacc;
-  try solve [inv_nuacc; eauto].
-  match goal with Hneq : _ <> ?ad |- _ =>
-    destruct (nat_eq_dec ad' ad); subst
-  end; inv_nuacc; simpl_array; eauto.
+  intros ** Huacc. induction Huacc; inv_nuacc; inv_nuacc; eauto.
+  match goal with _ : _ <> ?ad |- _ => destruct (nat_eq_dec ad' ad); subst end;
+  simpl_array; eauto.
 Qed.
 
 (* tstep ------------------------------------------------------------------- *)
@@ -111,38 +116,38 @@ Lemma nuacc_tstep_none_preservation : forall m t t' ad,
   t --[EF_None]--> t' ->
   ~ unsafe_access ad m t'.
 Proof.
-  intros. induction_tstep; inv_nuacc; trivial;
-  try solve [do 2 auto_specialize; intros ?; inv_uacc; eauto].
-  inv_nuacc. eauto using nuacc_subst_preservation. 
+  intros ** Huacc. induction_tstep; inv_nuacc;
+  try inv_uacc; eauto. inv_nuacc.
+  contradict Huacc. eauto using nuacc_subst_preservation.
 Qed.
 
 Lemma nuacc_tstep_alloc_preservation : forall m t t' ad v T,
-  ad < #m ->
   forall_memory m (valid_addresses m) ->
   valid_addresses m t ->
+  (* --- *)
+  ad < #m ->
   ~ unsafe_access ad m t ->
   t --[EF_Alloc (#m) v T]--> t' ->
   ~ unsafe_access ad (m +++ (v, T)) t'.
 Proof.
-  intros. intros ?. induction_tstep; inv_vad; inv_nuacc; invc_uacc; eauto;
+  intros ** ?. induction_tstep; inv_vad; inv_nuacc; invc_uacc; eauto;
   match goal with F : unsafe_access _ (_ +++ _) _ |- _ => contradict F end;
   try simpl_array;
   eauto using nacc_vad_length, nacc_then_nuacc, nuacc_mem_add_preservation.
 Qed.
 
-Lemma nuacc_tstep_read_preservation : forall m t t' ad ad' T,
+Lemma nuacc_tstep_read_preservation : forall m t t' ad ad',
   forall_memory m value ->
-  empty |-- t is T ->
+  well_typed_term t ->
   consistently_typed_references m t ->
+  (* --- *)
   ~ unsafe_access ad m t ->
   t --[EF_Read ad' m[ad'].tm]--> t' ->
   ~ unsafe_access ad m t'.
 Proof.
-  intros. intros ?. generalize dependent T.
-  induction_tstep; intros;
-  inv_type; inv_ctr; inv_nuacc; try invc_uacc; eauto;
-  inv_type; destruct (nat_eq_dec ad' ad); subst;
-  eauto using unsafe_access;
+  intros ** ?. induction_tstep; intros;
+  inv_wtt; inv_ctr; inv_nuacc; try invc_uacc; eauto;
+  inv_wtt; destruct (nat_eq_dec ad' ad); subst; eauto using unsafe_access;
   inv_ctr;
   match goal with F : unsafe_access _ _ _[_].tm |- _ => contradict F end;
   eauto using nuacc_from_immutable_type.
@@ -159,7 +164,7 @@ Proof.
     ~ unsafe_access ad m v)
     by (intros; induction_tstep; eauto using unsafe_access).
   (* main proof *)
-  intros. intros ?. induction_tstep; inv_nuacc; invc_uacc; eauto;
+  intros ** ?. induction_tstep; inv_nuacc; invc_uacc; eauto;
   match goal with _ : unsafe_access _ _ ?t |- _ => rename t into tx end;
   eapply (nuacc_mem_set_preservation _ tx _ _ v); eauto.
 Qed.
@@ -169,14 +174,16 @@ Lemma nuacc_tstep_spawn_preservation : forall m t t' ad block,
   t --[EF_Spawn block]--> t' ->
   ~ unsafe_access ad m t'.
 Proof.
-  intros. intros ?. induction_tstep; try inv_nuacc; inv_uacc; eauto.
+  intros ** ?. induction_tstep; inv_uacc; eauto; inv_nuacc; eauto.
 Qed.
 
-Local Corollary nuacc_mstep_preservation : forall m m' t t' e ad T,
+(* mstep ------------------------------------------------------------------- *)
+
+Corollary nuacc_mstep_preservation : forall m m' t t' e ad,
   forall_memory m value ->
   forall_memory m (valid_addresses m) ->
   valid_addresses m t ->
-  empty |-- t is T ->
+  well_typed_term t ->
   consistently_typed_references m t ->
   (* --- *)
   ad < #m ->
@@ -192,20 +199,20 @@ Proof.
 Qed.
 
 (* ------------------------------------------------------------------------- *)
-(*                                                                           *)
+(* misc. properties                                                          *)
 (* ------------------------------------------------------------------------- *)
 
-Lemma memtyp_mstep_nuacc_then_immut : forall m m' t t' e T,
-  empty |-- t is T ->
+Lemma memtyp_mstep_nuacc_then_immut : forall m m' t t' e,
+  well_typed_term t ->
   (* --- *)
   m / t ==[e]==> m' / t' ->
   #m' > #m ->
   ~ unsafe_access (#m) m' t' ->
   exists Tm, m'[#m].typ = <{{i&Tm}}>.
 Proof.
-  intros * ? ? Hlen. intros. invc_mstep;
+  intros * [T' ?] ? Hlen **. intros. invc_mstep;
   try rewrite set_preserves_length in Hlen; eauto.
-  simpl_array. simpl. generalize dependent T.
+  simpl_array. simpl. generalize dependent T'.
   induction_tstep; intros; inv_type; try inv_nuacc; eauto;
   try match goal with
   | _ : ?t --[_]--> _ , H : _ |-- ?t is _ |- _ =>
@@ -213,24 +220,24 @@ Proof.
   end.
 Qed.
 
-Lemma memtyp_mstep_uacc_then_mut : forall m m' t t' e T,
-  valid_accesses m t ->
-  empty |-- t is T ->
+Lemma memtyp_mstep_uacc_then_mut : forall m m' t t' e,
+  forall_memory m (valid_addresses m) ->
+  valid_addresses m t ->
+  well_typed_term t ->
   (* --- *)
   m / t ==[e]==> m' / t' ->
   #m' > #m ->
   unsafe_access (#m) m' t' ->
-  exists Tm, m'[#m].typ = <{{&Tm}}>.
+  exists T, m'[#m].typ = <{{&T}}>.
 Proof.
-  intros * ? ? ? Hlen. intros. invc_mstep;
+  intros * ? ? [T' ?] ? Hlen **. invc_mstep;
   try rewrite set_preserves_length in Hlen; eauto.
-  simpl_array. simpl. generalize dependent T.
-  induction_tstep; intros; inv_vac; inv_type; try invc_uacc;
-  eauto; exfalso;
+  simpl_array. simpl. generalize dependent T'.
+  induction_tstep; intros; inv_vad; inv_type; try invc_uacc; eauto; exfalso;
   match goal with
-  | H : valid_accesses _ ?t, _ : unsafe_access _ _ ?t |- _ =>
-    assert (~ access (#m) m t) by (intros F; specialize (H (#m) F); eauto)
+  | _ : unsafe_access _ _ ?t |- _ =>
+    assert (~ access (#m) m t) by eauto using nacc_vad_length
   end;
-  eauto using uacc_then_acc, InheritanceUACC.uacc_mem_add_inheritance.
+  eauto using uacc_then_acc, uacc_mem_add_inheritance.
 Qed.
 
