PropertiesVAD.v
@@ -49,210 +49,207 @@ Qed.
 (* preservation                                                              *)
 (* ------------------------------------------------------------------------- *)
 
-Module Preservation.
 
-  (* subst & mem ----------------------------------------------------------- *)
+(* subst & mem ------------------------------------------------------------- *)
 
-  Lemma vad_subst_preservation : forall m t tx x,
+Lemma vad_subst_preservation : forall m t tx x,
+  valid_addresses m t ->
+  valid_addresses m tx ->
+  valid_addresses m ([x := tx] t).
+Proof.
+  intros.
+  induction t; trivial; simpl; try solve [inv_vad; eauto with vad];
+  destruct string_eq_dec; subst; trivial. inv_vad. eauto with vad.
+Qed.
+
+Lemma vad_mem_add_preservation : forall m t vT,
+  valid_addresses m t ->
+  valid_addresses (m +++ vT) t.
+Proof.
+  intros. induction t; eauto with vad; inv_vad; eauto with vad.
+  intros ? ?. inv_hasad. rewrite add_increments_length. eauto.
+Qed.
+
+Lemma vad_mem_set_preservation : forall m t ad vT,
+  valid_addresses m t ->
+  valid_addresses m[ad <- vT] t.
+Proof.
+  intros. induction t; eauto with vad; inv_vad; eauto with vad.
+  intros ? ?. inv_hasad. rewrite set_preserves_length. assumption.
+Qed.
+
+(* tstep ------------------------------------------------------------------- *)
+
+Lemma vad_tstep_none_preservation : forall m t t',
+  valid_addresses m t ->
+  t --[EF_None]--> t' ->
+  valid_addresses m t'.
+Proof.
+  intros. induction_tstep; inv_vad; eauto with vad. 
+  inv_vad. eauto using vad_subst_preservation.
+Qed.
+
+Lemma vad_tstep_alloc_preservation : forall m t t' v T,
+  valid_addresses m t ->
+  t --[EF_Alloc (#m) v T]--> t' ->
+  valid_addresses (m +++ (v, T)) t'.
+Proof.
+  intros. induction_tstep; inv_vad;
+  eauto using vad_mem_add_preservation with vad.
+  intros ? ?. inv_hasad. rewrite add_increments_length. eauto.
+Qed.
+
+Lemma vad_tstep_read_preservation : forall m t t' ad v,
+  valid_addresses m v ->
+  valid_addresses m t ->
+  t --[EF_Read ad v]--> t' ->
+  valid_addresses m t'.
+Proof.
+  intros. induction_tstep; inv_vad; eauto with vad.
+Qed.
+
+Lemma vad_tstep_write_preservation : forall m t t' ad v T,
+  valid_addresses m t ->
+  t --[EF_Write ad v T]--> t' ->
+  valid_addresses m[ad <- (v, T)] t'.
+Proof.
+  intros. induction_tstep; inv_vad;
+  eauto using vad_mem_set_preservation with vad.
+Qed.
+
+Lemma vad_tstep_spawn_preservation : forall m t t' block,
+  valid_addresses m t ->
+  t --[EF_Spawn block]--> t' ->
+  valid_addresses m t'.
+Proof.
+  intros. induction_tstep; inv_vad; eauto with vad.
+Qed.
+
+(* mstep ------------------------------------------------------------------- *)
+
+Corollary vad_mstep_preservation : forall m m' t t' e,
+  forall_memory m (valid_addresses m) ->
+  valid_addresses m t ->
+  m / t ==[e]==> m' / t' ->
+  valid_addresses m' t'.
+Proof.
+  intros. inv_mstep;
+  eauto using vad_tstep_none_preservation,
+              vad_tstep_alloc_preservation,
+              vad_tstep_read_preservation,
+              vad_tstep_write_preservation.
+Qed.
+
+(* cstep ------------------------------------------------------------------- *)
+
+Lemma vad_thread_default : forall m,
+  valid_addresses m thread_default.
+Proof.
+  intros. eauto with vad.
+Qed.
+
+Lemma vad_spawn_block : forall m t t' block,
+  valid_addresses m t ->
+  t --[EF_Spawn block]--> t' ->
+  valid_addresses m block.
+Proof.
+  intros. induction_tstep; inv_vad; eauto.
+Qed.
+
+Lemma vad_untouched_threads_preservation : forall m m' ths tid tid' t' e,
+  forall_threads ths (valid_addresses m) ->
+  tid <> tid' ->
+  tid' < #ths ->
+  m / ths[tid] ==[e]==> m' / t' ->
+  valid_addresses m' ths[tid'].
+Proof.
+  intros. inv_mstep; 
+  eauto using vad_mem_add_preservation, vad_mem_set_preservation.
+Qed.
+
+Corollary vad_cstep_preservation : forall m m' ths ths' tid e,
+  forall_memory m (valid_addresses m) ->
+  forall_threads ths (valid_addresses m) ->
+  m / ths ~~[tid, e]~~> m' / ths' ->
+  forall_threads ths' (valid_addresses m').
+Proof.
+  intros. eauto 6 using cstep_preservation,
+    vad_tstep_spawn_preservation,
+    vad_mstep_preservation,
+    vad_thread_default,
+    vad_spawn_block,
+    vad_untouched_threads_preservation.
+Qed.
+
+(* tstep mem --------------------------------------------------------------- *)
+
+Lemma vad_tstep_alloc_mem_preservation : forall m t t' v T,
+  forall_memory m (valid_addresses m) ->
+  valid_addresses m t ->
+  t --[EF_Alloc (#m) v T]--> t' ->
+  forall_memory  (m +++ (v, T)) (valid_addresses (m +++ (v, T))).
+Proof.
+  assert (forall m t t' ad v T,
     valid_addresses m t ->
-    valid_addresses m tx ->
-    valid_addresses m ([x := tx] t).
-  Proof.
-    intros.
-    induction t; trivial; simpl; try solve [inv_vad; eauto with vad];
-    destruct string_eq_dec; subst; trivial. inv_vad. eauto with vad.
-  Qed.
+    t --[EF_Alloc ad v T]--> t' ->
+    valid_addresses m v)
+      by (intros; induction_tstep; inv_vad; eauto).
+  (* main proof *)
+  intros ** ad.
+  decompose sum (lt_eq_lt_dec ad (#m)); subst; simpl_array;
+  eauto using vad_mem_add_preservation with vad.
+Qed.
 
-  Lemma vad_mem_add_preservation : forall m t vT,
-    valid_addresses m t ->
-    valid_addresses (m +++ vT) t.
-  Proof.
-    intros. induction t; eauto with vad; inv_vad; eauto with vad.
-    intros ? ?. inv_hasad. rewrite add_increments_length. eauto.
-  Qed.
-
-  Lemma vad_mem_set_preservation : forall m t ad vT,
-    valid_addresses m t ->
-    valid_addresses m[ad <- vT] t.
-  Proof.
-    intros. induction t; eauto with vad; inv_vad; eauto with vad.
-    intros ? ?. inv_hasad. rewrite set_preserves_length. assumption.
-  Qed.
-
-  (* tstep ----------------------------------------------------------------- *)
-
-  Lemma vad_tstep_none_preservation : forall m t t',
-    valid_addresses m t ->
-    t --[EF_None]--> t' ->
-    valid_addresses m t'.
-  Proof.
-    intros. induction_tstep; inv_vad; eauto with vad. 
-    inv_vad. eauto using vad_subst_preservation.
-  Qed.
-
-  Lemma vad_tstep_alloc_preservation : forall m t t' v T,
-    valid_addresses m t ->
-    t --[EF_Alloc (#m) v T]--> t' ->
-    valid_addresses (m +++ (v, T)) t'.
-  Proof.
-    intros. induction_tstep; inv_vad;
-    eauto using vad_mem_add_preservation with vad.
-    intros ? ?. inv_hasad. rewrite add_increments_length. eauto.
-  Qed.
-
-  Lemma vad_tstep_read_preservation : forall m t t' ad v,
-    valid_addresses m v ->
-    valid_addresses m t ->
-    t --[EF_Read ad v]--> t' ->
-    valid_addresses m t'.
-  Proof.
-    intros. induction_tstep; inv_vad; eauto with vad.
-  Qed.
-
-  Lemma vad_tstep_write_preservation : forall m t t' ad v T,
+Lemma vad_tstep_write_mem_preservation : forall m t t' ad v T,
+  forall_memory m (valid_addresses m) ->
+  valid_addresses m t ->
+  t --[EF_Write ad v T]--> t' ->
+  forall_memory m[ad <- (v, T)] (valid_addresses m[ad <- (v, T)]).
+Proof.
+  assert (forall m t t' ad v T,
     valid_addresses m t ->
     t --[EF_Write ad v T]--> t' ->
-    valid_addresses m[ad <- (v, T)] t'.
-  Proof.
-    intros. induction_tstep; inv_vad;
-    eauto using vad_mem_set_preservation with vad.
-  Qed.
+    valid_addresses m v)
+      by (intros; induction_tstep; inv_vad; eauto).
+  (* main proof *)
+  intros ** ad'.
+  assert (ad < #m) by eauto using vad_tstep_write_address_length.
+  destruct (nat_eq_dec ad ad'); subst; simpl_array;
+  eauto using vad_mem_set_preservation.
+Qed.
 
-  Lemma vad_tstep_spawn_preservation : forall m t t' block,
-    valid_addresses m t ->
-    t --[EF_Spawn block]--> t' ->
-    valid_addresses m t'.
-  Proof.
-    intros. induction_tstep; inv_vad; eauto with vad.
-  Qed.
+(* mstep mem --------------------------------------------------------------- *)
 
-  (* mstep ----------------------------------------------------------------- *)
+Corollary vad_mstep_mem_preservation : forall m m' t t' e,
+  forall_memory m (valid_addresses m) ->
+  valid_addresses m t ->
+  m / t ==[e]==> m' / t' ->
+  forall_memory m' (valid_addresses m').
+Proof.
+  intros. inv_mstep;
+  eauto using vad_tstep_alloc_mem_preservation,
+              vad_tstep_write_mem_preservation.
+Qed.
 
-  Corollary vad_mstep_preservation : forall m m' t t' e,
-    forall_memory m (valid_addresses m) ->
-    valid_addresses m t ->
-    m / t ==[e]==> m' / t' ->
-    valid_addresses m' t'.
-  Proof.
-    intros. inv_mstep;
-    eauto using vad_tstep_none_preservation,
-                vad_tstep_alloc_preservation,
-                vad_tstep_read_preservation,
-                vad_tstep_write_preservation.
-  Qed.
+(* cstep mem --------------------------------------------------------------- *)
 
-  (* cstep ----------------------------------------------------------------- *)
+Corollary vad_cstep_mem_preservation : forall m m' ths ths' tid e,
+  forall_memory m (valid_addresses m) ->
+  forall_threads ths (valid_addresses m) ->
+  m / ths ~~[tid, e]~~> m' / ths' ->
+  forall_memory m' (valid_addresses m').
+Proof.
+  intros. inv_cstep; eauto using vad_mstep_mem_preservation.
+Qed.
 
-  Lemma vad_thread_default : forall m,
-    valid_addresses m thread_default.
-  Proof.
-    intros. eauto with vad.
-  Qed.
+(* valid-addresses preservation -------------------------------------------- *)
 
-  Lemma vad_spawn_block : forall m t t' block,
-    valid_addresses m t ->
-    t --[EF_Spawn block]--> t' ->
-    valid_addresses m block.
-  Proof.
-    intros. induction_tstep; inv_vad; eauto.
-  Qed.
-
-  Lemma vad_untouched_threads_preservation : forall m m' ths tid tid' t' e,
-    forall_threads ths (valid_addresses m) ->
-    tid <> tid' ->
-    tid' < #ths ->
-    m / ths[tid] ==[e]==> m' / t' ->
-    valid_addresses m' ths[tid'].
-  Proof.
-    intros. inv_mstep; 
-    eauto using vad_mem_add_preservation, vad_mem_set_preservation.
-  Qed.
-
-  Corollary vad_cstep_preservation : forall m m' ths ths' tid e,
-    forall_memory m (valid_addresses m) ->
-    forall_threads ths (valid_addresses m) ->
-    m / ths ~~[tid, e]~~> m' / ths' ->
-    forall_threads ths' (valid_addresses m').
-  Proof.
-    intros. eauto 6 using cstep_preservation,
-      vad_tstep_spawn_preservation,
-      vad_mstep_preservation,
-      vad_thread_default,
-      vad_spawn_block,
-      vad_untouched_threads_preservation.
-  Qed.
-
-  (* tstep mem ------------------------------------------------------------- *)
-
-  Lemma vad_tstep_alloc_mem_preservation : forall m t t' v T,
-    forall_memory m (valid_addresses m) ->
-    valid_addresses m t ->
-    t --[EF_Alloc (#m) v T]--> t' ->
-    forall_memory  (m +++ (v, T)) (valid_addresses (m +++ (v, T))).
-  Proof.
-    assert (forall m t t' ad v T,
-      valid_addresses m t ->
-      t --[EF_Alloc ad v T]--> t' ->
-      valid_addresses m v)
-        by (intros; induction_tstep; inv_vad; eauto).
-    (* main proof *)
-    intros ** ad.
-    decompose sum (lt_eq_lt_dec ad (#m)); subst; simpl_array;
-    eauto using vad_mem_add_preservation with vad.
-  Qed.
-
-  Lemma vad_tstep_write_mem_preservation : forall m t t' ad v T,
-    forall_memory m (valid_addresses m) ->
-    valid_addresses m t ->
-    t --[EF_Write ad v T]--> t' ->
-    forall_memory m[ad <- (v, T)] (valid_addresses m[ad <- (v, T)]).
-  Proof.
-    assert (forall m t t' ad v T,
-      valid_addresses m t ->
-      t --[EF_Write ad v T]--> t' ->
-      valid_addresses m v)
-        by (intros; induction_tstep; inv_vad; eauto).
-    (* main proof *)
-    intros ** ad'.
-    assert (ad < #m) by eauto using vad_tstep_write_address_length.
-    destruct (nat_eq_dec ad ad'); subst; simpl_array;
-    eauto using vad_mem_set_preservation.
-  Qed.
-
-  (* mstep mem ------------------------------------------------------------- *)
-
-  Corollary vad_mstep_mem_preservation : forall m m' t t' e,
-    forall_memory m (valid_addresses m) ->
-    valid_addresses m t ->
-    m / t ==[e]==> m' / t' ->
-    forall_memory m' (valid_addresses m').
-  Proof.
-    intros. inv_mstep;
-    eauto using vad_tstep_alloc_mem_preservation,
-                vad_tstep_write_mem_preservation.
-  Qed.
-
-  (* cstep mem ------------------------------------------------------------- *)
-
-  Corollary vad_cstep_mem_preservation : forall m m' ths ths' tid e,
-    forall_memory m (valid_addresses m) ->
-    forall_threads ths (valid_addresses m) ->
-    m / ths ~~[tid, e]~~> m' / ths' ->
-    forall_memory m' (valid_addresses m').
-  Proof.
-    intros. inv_cstep; eauto using vad_mstep_mem_preservation.
-  Qed.
-
-  (* valid-addresses preservation ------------------------------------------ *)
-
-  Theorem valid_addresses_preservation : forall m m' ths ths' tid e,
-    forall_program m ths (valid_addresses m) ->
-    m / ths ~~[tid, e]~~> m' / ths' ->
-    forall_program m' ths' (valid_addresses m').
-  Proof.
-    intros * [? ?] **.
-    eauto using vad_cstep_preservation, vad_cstep_mem_preservation.
-  Qed.
-
-End Preservation.
+Theorem valid_addresses_preservation : forall m m' ths ths' tid e,
+  forall_program m ths (valid_addresses m) ->
+  m / ths ~~[tid, e]~~> m' / ths' ->
+  forall_program m' ths' (valid_addresses m').
+Proof.
+  intros * [? ?] **.
+  eauto using vad_cstep_preservation, vad_cstep_mem_preservation.
+Qed.
 
