Sanity.v
@@ -1,0 +1,6 @@
+From Elo Require Import Util.
+From Elo Require Import Core.
+
+From Elo Require Import Definitions.
+
+(* TODO: has-address *)
